Adjust eval_expr and typecheck_expr to permit by-reference lvalues to serve as exprs (rvalues); install a version of progs/test1.v (almost) as produced by CompCert clightgen from test1.c, and (almost) prove it correct in separation logic

progs/test1.v
@@ -1,144 +1,172 @@
-Load loadpath.
-(* 
-#include <stddef.h>
+Require Import Clightdefs.
 
-struct list {int h; struct list *t;};
+Local Open Scope Z_scope.
 
-struct list three[] = {
-    {1, three+1}, {2, three+2}, {3, NULL}
-};
+Definition _main : ident := 15%positive.
+Definition _h : ident := 7%positive.
+Definition ___builtin_annot_intval : ident := 3%positive.
+Definition ___builtin_fabs : ident := 1%positive.
+Definition _r : ident := 14%positive.
+Definition _s : ident := 9%positive.
+Definition _three : ident := 4%positive.
+Definition _p : ident := 8%positive.
+Definition _reverse : ident := 13%positive.
+Definition _t : ident := 6%positive.
+Definition _v : ident := 12%positive.
+Definition _w : ident := 11%positive.
+Definition _struct_list : ident := 5%positive.
+Definition ___builtin_memcpy_aligned : ident := 2%positive.
+Definition _sumlist : ident := 10%positive.
 
-int sumlist (struct list *p) {
-  int s = 0;
-  struct list *t = p;
-  int h;
-  while (t) {
-     h = t->h;
-     t = t->t;
-     s = s + h;
-  }
-  return s;
-}
+Definition t_struct_list :=
+   (Tstruct _struct_list
+     (Fcons _h tint (Fcons _t (Tcomp_ptr _struct_list noattr) Fnil)) noattr).
 
-struct list *reverse (struct list *p) {
-  struct list *w, *t, *v;
-  w = NULL; 
-  v = p;
-  while (v) {
-    t = v->t;
-    v->t = w;
-    w = v;
-    v = t;
-  }
-  return w;
-}  
+Definition v_three := {|
+  gvar_info := (tarray t_struct_list 3);
+  gvar_init := (Init_int32 (Int.repr 1) :: Init_addrof _three (Int.repr 8) ::
+                Init_int32 (Int.repr 2) ::
+                Init_addrof _three (Int.repr 16) ::
+                Init_int32 (Int.repr 3) :: Init_int32 (Int.repr 0) :: nil);
+  gvar_readonly := false;
+  gvar_volatile := false
+|}.
 
-int main (void) {
-  struct list *r; int s;
-  r = reverse(three);
-  s = sumlist(r);
-  return s;
-}
+Definition f_sumlist := {|
+  fn_return := tint;
+  fn_params := ((_p, (tptr t_struct_list)) :: nil);
+  fn_vars := nil;
+  fn_temps := ((_s, tint) :: (_t, (tptr t_struct_list)) :: (_h, tint) :: nil);
+  fn_body :=
+(Ssequence
+  (Sset _s (Ecast (Econst_int (Int.repr 0) tint) tint))
+  (Ssequence
+    (Sset _t (Ecast (Etempvar _p (tptr t_struct_list)) (tptr t_struct_list)))
+    (Ssequence
+      (Swhile
+        (Etempvar _t (tptr t_struct_list))
+        (Ssequence
+          (Sset _h
+            (Ecast
+              (Efield
+                (Ederef (Etempvar _t (tptr t_struct_list)) t_struct_list) _h
+                tint) tint))
+          (Ssequence
+            (Sset _t
+              (Ecast
+                (Efield
+                  (Ederef (Etempvar _t (tptr t_struct_list)) t_struct_list)
+                  _t (tptr t_struct_list)) (tptr t_struct_list)))
+            (Sset _s
+              (Ecast (Ebinop Oadd (Etempvar _s tint) (Etempvar _h tint) tint)
+                tint)))))
+      (Sreturn (Some (Etempvar _s tint))))))
+|}.
+
+Definition f_reverse := {|
+  fn_return := (tptr t_struct_list);
+  fn_params := ((_p, (tptr t_struct_list)) :: nil);
+  fn_vars := nil;
+  fn_temps := ((_w, (tptr t_struct_list)) :: (_t, (tptr t_struct_list)) ::
+               (_v, (tptr t_struct_list)) :: nil);
+  fn_body :=
+(Ssequence
+  (Sset _w
+    (Ecast (Ecast (Econst_int (Int.repr 0) tint) (tptr tvoid))
+      (tptr t_struct_list)))
+  (Ssequence
+    (Sset _v (Ecast (Etempvar _p (tptr t_struct_list)) (tptr t_struct_list)))
+    (Ssequence
+      (Swhile
+        (Etempvar _v (tptr t_struct_list))
+        (Ssequence
+          (Sset _t
+            (Ecast
+              (Efield
+                (Ederef (Etempvar _v (tptr t_struct_list)) t_struct_list) _t
+                (tptr t_struct_list)) (tptr t_struct_list)))
+          (Ssequence
+            (Sassign
+              (Efield
+                (Ederef (Etempvar _v (tptr t_struct_list)) t_struct_list) _t
+                (tptr t_struct_list)) (Etempvar _w (tptr t_struct_list)))
+            (Ssequence
+              (Sset _w
+                (Ecast (Etempvar _v (tptr t_struct_list))
+                  (tptr t_struct_list)))
+              (Sset _v
+                (Ecast (Etempvar _t (tptr t_struct_list))
+                  (tptr t_struct_list)))))))
+      (Sreturn (Some (Etempvar _w (tptr t_struct_list)))))))
+|}.
+
+(* as produced by Clightgen, version as of 6 jan 2012 ...
+Definition f_main := {|
+  fn_return := tint;
+  fn_params := nil;
+  fn_vars := nil;
+  fn_temps := ((_r, (tptr t_struct_list)) :: (_s, tint) ::
+               (17%positive, tint) :: (16%positive, (tptr t_struct_list)) ::
+               nil);
+  fn_body :=
+(Ssequence
+  (Ssequence
+    (Scall (Some 16%positive)
+      (Evar _reverse (Tfunction (Tcons (tptr t_struct_list) Tnil)
+                       (tptr t_struct_list)))
+      ((Evar _three (tarray t_struct_list 3)) :: nil))
+    (Sset _r
+      (Ecast (Etempvar 16%positive (tptr t_struct_list))
+        (tptr t_struct_list))))
+  (Ssequence
+    (Ssequence
+      (Scall (Some 17%positive)
+        (Evar _sumlist (Tfunction (Tcons (tptr t_struct_list) Tnil) tint))
+        ((Etempvar _r (tptr t_struct_list)) :: nil))
+      (Sset _s (Ecast (Etempvar 17%positive tint) tint)))
+    (Sreturn (Some (Etempvar _s tint)))))
+|}.
 *)
-Require Import veric.base.
-Require Import Maps.
-Import Cop.
 
-Section idents.
-Local Open Scope positive_scope.
-Definition i_s : ident := 1.
-Definition i_h : ident := 2.
-Definition i_t : ident := 3.
-Definition i_list : ident := 4.
-Definition i_sumlist : ident := 5.
-Definition i_p : ident := 6.
-Definition i_three : ident := 7.
-Definition i_reverse : ident := 8.
-Definition i_w : ident := 9.
-Definition i_v : ident := 10.
-Definition i_main : ident := 11.
-Definition i_r : ident := 12.
-End idents.
+Definition f_main := {|
+  fn_return := tint;
+  fn_params := nil;
+  fn_vars := nil;
+  fn_temps := ((_r, (tptr t_struct_list)) :: (_s, tint) :: nil);
+  fn_body :=
+(Ssequence
+    (Scall (Some _r)
+      (Evar _reverse (Tfunction (Tcons (tptr t_struct_list) Tnil)
+                       (tptr t_struct_list)))
+      ((Evar _three (tarray t_struct_list 3)) :: nil))
+  (Ssequence
+      (Scall (Some _s)
+        (Evar _sumlist (Tfunction (Tcons (tptr t_struct_list) Tnil) tint))
+        ((Etempvar _r (tptr t_struct_list)) :: nil))
+    (Sreturn (Some (Etempvar _s tint)))))
+|}.
 
-Definition t_int := Tint I32 Signed noattr.
+Definition prog : Clight.program := {|
+prog_defs :=
+((___builtin_fabs,
+   Gfun(External (EF_builtin ___builtin_fabs
+                   (mksignature (AST.Tfloat :: nil) (Some AST.Tfloat)))
+     (Tcons tdouble Tnil) tdouble)) ::
+ (___builtin_memcpy_aligned,
+   Gfun(External (EF_builtin ___builtin_memcpy_aligned
+                   (mksignature
+                     (AST.Tint :: AST.Tint :: AST.Tint :: AST.Tint :: nil)
+                     None))
+     (Tcons (tptr tvoid)
+       (Tcons (tptr tvoid) (Tcons tuint (Tcons tuint Tnil)))) tvoid)) ::
+ (___builtin_annot_intval,
+   Gfun(External (EF_builtin ___builtin_annot_intval
+                   (mksignature (AST.Tint :: AST.Tint :: nil)
+                     (Some AST.Tint)))
+     (Tcons (tptr tschar) (Tcons tint Tnil)) tint)) ::
+ (_three, Gvar v_three) :: (_sumlist, Gfun(Internal f_sumlist)) ::
+ (_reverse, Gfun(Internal f_reverse)) :: (_main, Gfun(Internal f_main)) ::
+ nil);
+prog_main := _main
+|}.
 
-Definition t_list :=   Tstruct i_list (Fcons i_h t_int
-               (Fcons i_t (Tcomp_ptr i_list noattr)
-               Fnil)) noattr.
-
-Definition t_listptr := Tpointer t_list noattr.
-Definition t_voidptr := Tpointer Tvoid noattr.
-
-Definition set: forall {A}, ident -> A -> PTree.t A -> PTree.t A := 
- @PTree.set.
-Implicit Arguments set [A].
-
-Definition zet {A} (i: Z) (x: A) (m: ZMap.t (option A)) : ZMap.t (option A) := 
- ZMap.set i (Some x) m.
-Implicit Arguments zet [A].
-
-Definition f_sumlist : function :=
-  mkfunction
- (* return *) t_int
- (* params *) ((i_p, t_listptr)::nil)
- (* vars *)  nil
- (* temps *) ((i_s,t_int)::(i_t,t_listptr)::(i_h,t_int)::nil)
- (* body *) 
-  (Ssequence (Sset i_s (Econst_int (Int.repr 0) t_int))
-   (Ssequence (Sset i_t (Etempvar i_p t_listptr))
-    (  (* Ssequence (Sset i_h (Econst_int (Int.repr 0) t_int)) *)
-     (Ssequence 
-         (Swhile (Etempvar i_t t_listptr)
-          (Ssequence (Sset i_h (Efield (Ederef (Etempvar i_t t_listptr) t_list) i_h t_int))
-           (Ssequence (Sset i_t (Efield (Ederef (Etempvar i_t t_listptr) t_list) i_t t_listptr))
-            (Sset i_s (Ebinop Oadd (Etempvar i_s t_int) (Etempvar i_h t_int) t_int)))))
-   (Sreturn (Some (Etempvar i_s t_int))))))).
-
-Definition f_reverse: function :=
- mkfunction
- (* return *) t_listptr
- (* params *) ((i_p, t_listptr)::nil)
- (* vars *)  nil
- (* temps *) ((i_w,t_listptr)::(i_t,t_listptr)::(i_v,t_listptr)::nil)
- (* body *) 
-  (Ssequence (Sset i_w (Ecast (Ecast (Econst_int (Int.repr 0) t_int) t_voidptr) (t_listptr)))
-   (Ssequence (Sset i_v (Etempvar i_p t_listptr))
-    (Ssequence 
-         (Swhile (Etempvar i_v t_listptr)
-          (Ssequence (Sset i_t (Efield (Ederef (Etempvar i_v t_listptr) t_list) i_t t_listptr))
-           (Ssequence (Sassign (Efield (Ederef (Etempvar i_v t_listptr) t_list) i_t t_listptr) (Etempvar i_w t_listptr))
-           (Ssequence (Sset i_w (Etempvar i_v t_listptr))
-            (Sset i_v (Etempvar i_t t_listptr))))))
-   (Sreturn (Some (Etempvar i_w t_listptr)))))).
-
-Definition f_main: function :=
- mkfunction
- (* return *) t_int
- (* params *) nil
- (* vars *)  nil
- (* temps *)  ((i_r, t_listptr)::(i_s, t_int)::nil) 
- (* body *) 
-  (Ssequence (Scall (Some i_r) 
-                        (Eaddrof (Evar i_reverse (Tfunction (Tcons t_listptr Tnil) t_listptr))
-                                   (Tpointer (Tfunction (Tcons t_listptr Tnil) t_listptr) noattr))
-                        (Ecast (Eaddrof (Evar i_three (Tarray t_list 3 noattr)) (Tpointer (Tarray t_list 3 noattr) noattr)) t_listptr :: nil))
-    (Ssequence (Scall (Some i_s) 
-                           (Eaddrof (Evar i_sumlist (Tfunction (Tcons t_listptr Tnil) t_int))
-                                             (Tpointer  (Tfunction (Tcons t_listptr Tnil) t_int)  noattr))
-                          (Etempvar i_r t_listptr::nil)) 
-     (Sreturn (Some (Etempvar i_s t_int))))).
-
-Definition gv_three : globvar type :=
-  mkglobvar (Tarray t_list 3 noattr)
-       (Init_int32 (Int.repr 1) :: Init_addrof i_three (Int.repr 8) ::
-        Init_int32 (Int.repr 2) :: Init_addrof i_three (Int.repr 16) ::
-        Init_int32 (Int.repr 3) :: Init_int32 (Int.repr 0) ::
-        nil)
-        false
-        false.
-
-Definition prog : program :=
-  mkprogram ((i_sumlist, Gfun (Internal f_sumlist))::(i_reverse, Gfun (Internal f_reverse))
-                            ::(i_main, Gfun (Internal f_main))
-                            ::(i_three, Gvar gv_three)::nil)
-                      i_main.
